Strengthen OFFSET well-formedness contract

venom/defs/venomWfScript.sml
@@ -156,8 +156,8 @@ Definition inst_wf_def:
     | CREATE => LENGTH inst.inst_operands = 3 ∧ LENGTH inst.inst_outputs = 1
     | CREATE2 => LENGTH inst.inst_operands = 4 ∧ LENGTH inst.inst_outputs = 1
     (* ---- Special ---- *)
-    | OFFSET => ∃op lbl. inst.inst_operands = [op; Label lbl] ∧
-                         LENGTH inst.inst_outputs = 1
+    | OFFSET => ∃v lbl. inst.inst_operands = [Lit v; Label lbl] ∧
+                        LENGTH inst.inst_outputs = 1
     | LOG => ∃tc rest. inst.inst_operands = Lit tc :: rest ∧
                        LENGTH rest = w2n tc + 2 /\ inst.inst_outputs = []
     | SELFDESTRUCT => LENGTH inst.inst_operands = 1 /\ inst.inst_outputs = []
@@ -169,6 +169,18 @@ Definition inst_wf_def:
        arity which can be 0, 1, or more - see check_venom._collect_ret_arities) ---- *)
     | INVOKE => ∃lbl args. inst.inst_operands = Label lbl :: args
 End
+
+Theorem inst_wf_offset_shape:
+  inst_wf inst /\ inst.inst_opcode = OFFSET ==>
+  ?v lbl out.
+    inst.inst_operands = [Lit v; Label lbl] /\
+    inst.inst_outputs = [out]
+Proof
+  rpt strip_tac >>
+  gvs[inst_wf_def] >>
+  Cases_on `inst.inst_outputs` >> gvs[] >>
+  Cases_on `t` >> gvs[]
+QED
 
 (* The function has an entry block (fn_blocks is non-empty). *)
 Definition fn_has_entry_def:
